use variable for type A

TextOperation.v
@@ -5,23 +5,27 @@ Require Import
   Coq.Strings.String
   Coq.Lists.List.
 
+Section TextOperation.
+
+Variable A : Type.
+
 Local Notation "[ ]" := nil : list_scope.
 Local Notation "[ a ; .. ; b ]" := (a :: .. (b :: []) ..) : list_scope.
 (* Import ListNotations. *) (* in Coq 8.4 *)
 
-Inductive ListOperation (A : Type) : Type :=
-  | EmptyOp  : ListOperation A
-  | RetainOp : ListOperation A -> ListOperation A
-  | InsertOp : A -> ListOperation A -> ListOperation A
-  | DeleteOp : ListOperation A -> ListOperation A.
+Inductive ListOperation : Type :=
+  | EmptyOp  : ListOperation
+  | RetainOp : ListOperation -> ListOperation
+  | InsertOp : A -> ListOperation -> ListOperation
+  | DeleteOp : ListOperation -> ListOperation.
 
-Inductive ListOperationLength {A : Type} : ListOperation A -> nat -> nat -> Prop :=
-  | LengthEmpty  : ListOperationLength (EmptyOp A) 0 0
-  | LengthRetain : forall o n m, ListOperationLength o n m -> ListOperationLength (RetainOp A o) (S n) (S m)
-  | LengthInsert : forall a o n m, ListOperationLength o n m -> ListOperationLength (InsertOp A a o) n (S m)
-  | LengthDelete : forall o n m, ListOperationLength o n m -> ListOperationLength (DeleteOp A o) (S n) m.
+Inductive ListOperationLength : ListOperation -> nat -> nat -> Prop :=
+  | LengthEmpty  : ListOperationLength EmptyOp 0 0
+  | LengthRetain : forall o n m, ListOperationLength o n m -> ListOperationLength (RetainOp o) (S n) (S m)
+  | LengthInsert : forall a o n m, ListOperationLength o n m -> ListOperationLength (InsertOp a o) n (S m)
+  | LengthDelete : forall o n m, ListOperationLength o n m -> ListOperationLength (DeleteOp o) (S n) m.
 
-Fixpoint apply {A : Type} (o : ListOperation A) (l : list A) : option (list A) :=
+Fixpoint apply (o : ListOperation) (l : list A) : option (list A) :=
   match o, l with
   | EmptyOp,       []      => Some []
   | RetainOp o',   x :: xs => option_map (fun xs' => x :: xs') (apply o' xs)
@@ -30,11 +34,11 @@ Fixpoint apply {A : Type} (o : ListOperation A) (l : list A) : option (list A) :
   | _,             _       => None
   end.
 
-Theorem apply_length : forall {A : Type} (o : ListOperation A) (l : list A) (m : nat),
+Theorem apply_length : forall (o : ListOperation) (l : list A) (m : nat),
   ListOperationLength o (length l) m ->
   exists l', apply o l = Some l' /\ length l' = m.
 Proof with auto.
-  intros A o. induction o; intros.
+  intros o. induction o; intros.
     inversion H. destruct l.
       exists []...
       inversion H0.
@@ -53,15 +57,15 @@ Proof with auto.
         assumption.
 Qed.
 
-Fixpoint compose {A : Type} (a : ListOperation A) : ListOperation A -> option (ListOperation A) :=
-  fix compose' (b : ListOperation A) : option (ListOperation A) :=
+Fixpoint compose (a : ListOperation) : ListOperation -> option ListOperation :=
+  fix compose' (b : ListOperation) : option (ListOperation) :=
     match a, b with
-    | EmptyOp,       EmptyOp       => Some (EmptyOp A)
-    | DeleteOp a',   _             => option_map (DeleteOp A)   (compose a' b)
-    | _,             InsertOp c b' => option_map (InsertOp A c) (compose' b')
-    | RetainOp a',   RetainOp b'   => option_map (RetainOp A)   (compose a' b')
-    | RetainOp a',   DeleteOp b'   => option_map (DeleteOp A)   (compose a' b')
-    | InsertOp c a', RetainOp b'   => option_map (InsertOp A c) (compose a' b')
+    | EmptyOp,       EmptyOp       => Some (EmptyOp)
+    | DeleteOp a',   _             => option_map DeleteOp     (compose a' b)
+    | _,             InsertOp c b' => option_map (InsertOp c) (compose' b')
+    | RetainOp a',   RetainOp b'   => option_map RetainOp     (compose a' b')
+    | RetainOp a',   DeleteOp b'   => option_map DeleteOp     (compose a' b')
+    | InsertOp c a', RetainOp b'   => option_map (InsertOp c) (compose a' b')
     | InsertOp _ a', DeleteOp b'   => compose a' b'
     | _,             _             => None
     end.
@@ -72,43 +76,19 @@ Definition pair_map {A A' B B' : Type} (f : A -> A') (g : B -> B') (p : A * B) :
 Definition option_pair_map {A A' B B' : Type} (f : A -> A') (g : B -> B') (mp : option (A * B)) : option (A' * B') :=
   option_map (pair_map f g) mp.
 
-Fixpoint transform {A : Type} (a : ListOperation A) : ListOperation A -> option (ListOperation A * ListOperation A) :=
-  fix transform' (b : ListOperation A) : option (ListOperation A * ListOperation A) :=
+Fixpoint transform (a : ListOperation) : ListOperation -> option (ListOperation * ListOperation) :=
+  fix transform' (b : ListOperation) : option (ListOperation * ListOperation) :=
     match a, b with
-    | EmptyOp,       EmptyOp       => Some (pair (EmptyOp A) (EmptyOp A))
-    | InsertOp c a', _             => option_pair_map (InsertOp A c) (RetainOp A)   (transform a' b)
-    | _,             InsertOp c b' => option_pair_map (RetainOp A)   (InsertOp A c) (transform' b')
-    | RetainOp a',   RetainOp b'   => option_pair_map (RetainOp A)   (RetainOp A)   (transform a' b')
+    | EmptyOp,       EmptyOp       => Some (pair EmptyOp EmptyOp)
+    | InsertOp c a', _             => option_pair_map (InsertOp c) RetainOp     (transform a' b)
+    | _,             InsertOp c b' => option_pair_map RetainOp     (InsertOp c) (transform' b')
+    | RetainOp a',   RetainOp b'   => option_pair_map RetainOp     RetainOp     (transform a' b')
     | DeleteOp a',   DeleteOp b'   => transform a' b'
-    | RetainOp a',   DeleteOp b'   => option_pair_map (DeleteOp A)   (fun x => x)   (transform a' b')
-    | DeleteOp a',   RetainOp b'   => option_pair_map (fun x => x)   (DeleteOp A)   (transform a' b')
+    | RetainOp a',   DeleteOp b'   => option_pair_map DeleteOp     (fun x => x) (transform a' b')
+    | DeleteOp a',   RetainOp b'   => option_pair_map (fun x => x) DeleteOp     (transform a' b')
     | _,             _             => None
     end.
 
-(*
-Inductive ListOperation (A : Type) : nat -> nat -> Type :=
-  | EmptyOp  : ListOperation A 0 0
-  | RetainOp : forall n m, ListOperation A n m -> ListOperation A (S n) (S m)
-  | InsertOp : forall n m, A -> ListOperation A n m -> ListOperation A n (S m)
-  | DeleteOp : forall n m, ListOperation A n m -> ListOperation A (S n) m.
-
-Definition TextOperation := ListOperation ascii.
-
-Local Open Scope vector_scope.
-
-Fixpoint apply {A : Type} {n m : nat} (o : ListOperation A n m) (v : t A n) : t A m :=
-  match o with
-  | EmptyOp => nil A (*[]%vector_scope nil []*)
-  | RetainOp (S n) (S m) o' => match v with
-    | cons x _ xs => cons x (apply o' xs)
-    end
-  | InsertOp n (S m) a o' => cons a _ (apply o' v)
-  | DeleteOp (S n) m o' => match v with
-    | cons _ _ xs => apply o' xs
-    end
-  end.
-
-Fixpoint compose {A : Type} {n m k : nat} (a : ListOperation A n m) (b : ListOperation A m k) : ListOperation A n k := Admit.
-*)
+End TextOperation.
 
 End TextOperation.
